theories/examples/sort_elem_client.v
@@ -3,7 +3,7 @@ From osiris.channel Require Import proto_channel proofmode.
 From iris.heap_lang Require Import proofmode notation.
 From iris.heap_lang Require Import assert.
 From osiris.utils Require Import list compare.
-From osiris.examples Require Import list_sort_elem.
+From osiris.examples Require Import sort_elem.
 
 Definition send_all : val :=
   rec: "go" "c" "xs" :=
@@ -18,21 +18,21 @@ Definition recv_all : val :=
     then let: "x" := recv "c" in lcons "x" ("go" "c")
     else lnil #().
 
-Definition list_sort_elem_client : val :=
+Definition sort_elem_client : val :=
   λ: "cmp" "xs",
-    let: "c" := start_chan list_sort_elem_service_top in
+    let: "c" := start_chan sort_elem_service_top in
     send "c" "cmp";;
     send_all "c" "xs";;
     recv_all "c".
 
-Section list_sort_elem_client.
+Section sort_elem_client.
   Context `{!heapG Σ, !proto_chanG Σ} (N : namespace).
   Context {A} (I : A → val → iProp Σ) (R : relation A) `{!RelDecision R, !Total R}.
 
   Lemma send_all_spec c p xs' xs vs :
-    {{{ c ↣ head_protocol I R xs' <++> p @ N ∗ [∗ list] x;v ∈ xs;vs, I x v }}}
+    {{{ c ↣ sort_elem_head_protocol I R xs' <++> p @ N ∗ [∗ list] x;v ∈ xs;vs, I x v }}}
       send_all c (val_encode vs)
-    {{{ RET #(); c ↣ tail_protocol I R (xs' ++ xs) [] <++> p @ N }}}.
+    {{{ RET #(); c ↣ sort_elem_tail_protocol I R (xs' ++ xs) [] <++> p @ N }}}.
   Proof.
     iIntros (Φ) "[Hc HI] HΦ".
     iInduction xs as [|x xs] "IH" forall (xs' vs); destruct vs as [|v vs]=>//.
@@ -44,7 +44,7 @@ Section list_sort_elem_client.
 
   Lemma recv_all_spec c p xs ys' :
     Sorted R ys' →
-    {{{ c ↣ tail_protocol I R xs ys' <++> p @ N }}}
+    {{{ c ↣ sort_elem_tail_protocol I R xs ys' <++> p @ N }}}
       recv_all c
     {{{ ys ws, RET (val_encode ws);
         ⌜Sorted R (ys' ++ ys)⌝ ∗ ⌜ys' ++ ys ≡ₚ xs⌝ ∗
@@ -63,22 +63,22 @@ Section list_sort_elem_client.
       iApply ("HΦ" $! [] []); rewrite /= right_id_L; by iFrame.
   Qed.
 
-  Lemma list_sort_client_spec cmp vs xs :
+  Lemma sort_client_spec cmp vs xs :
     cmp_spec I R cmp -∗
     {{{ [∗ list] x;v ∈ xs;vs, I x v }}}
-      list_sort_elem_client cmp (val_encode vs)
+      sort_elem_client cmp (val_encode vs)
     {{{ ys ws, RET (val_encode ws); ⌜Sorted R ys⌝ ∗ ⌜ys ≡ₚ xs⌝ ∗
                [∗ list] y;w ∈ ys;ws, I y w }}}.
   Proof.
     iIntros "#Hcmp !>" (Φ) "HI HΦ". wp_lam.
-    wp_apply (start_chan_proto_spec N (list_sort_elem_top_protocol <++> END)%proto);
+    wp_apply (start_chan_proto_spec N (sort_elem_top_protocol <++> END)%proto);
       iIntros (c) "Hc".
-    { wp_apply (list_sort_elem_service_top_spec N with "Hc"); auto. }
-    rewrite /list_sort_elem_top_protocol.
+    { wp_apply (sort_elem_service_top_spec N with "Hc"); auto. }
+    rewrite /sort_elem_top_protocol.
     wp_send (A I R) with "[$Hcmp]".
     wp_apply (send_all_spec with "[$HI $Hc]"); iIntros "Hc".
     wp_apply (recv_all_spec _ _ _ [] with "[$Hc]"); auto.
     iIntros (ys ws) "/=". iDestruct 1 as (??) "[_ HI]".
     iApply "HΦ"; auto.
   Qed.
-End list_sort_elem_client.
+End sort_elem_client.
